{-# OPTIONS  #-}

open import Base
open import Integers

module Spaces.FlatteningLoopSpaceWedgeCircles {i} (A : Set i) (set : is-set A)
  where

import Spaces.WedgeCircles
import Algebra.FreeGroup
import Algebra.FreeGroupProps
import Algebra.FreeGroupAsReducedWords

open Spaces.WedgeCircles A renaming (wedge-circles to WA; base to baseWA)
open Algebra.FreeGroup A renaming (freegroup to FA)
open Algebra.FreeGroupProps A

-- Path fibration

path-fib : WA → Set (suc i)
path-fib t = (t ≡ baseWA)

tot-path-fib : Set (suc i)
tot-path-fib = Σ (WA) path-fib

abstract
  tot-path-fib-is-contr : is-contr tot-path-fib
  tot-path-fib-is-contr = pathto-is-contr baseWA

-- Universal cover

x·-path : A → FA ≡ FA
x·-path x = eq-to-path (_ , x·-is-equiv x)

universal-cover : WA → Set i
universal-cover = wedge-circles-rec-nondep (Set _) FA x·-path

tot-cover : Set _
tot-cover = Σ WA universal-cover

trans-universal-cover : {u v : WA} (p : u ≡ v) (q : universal-cover u)
  → transport universal-cover p q
    ≡ transport (λ A → A) (ap universal-cover p) q
trans-universal-cover refl _ = refl

abstract
  loops-to-x· : (t : A) (u : FA) → transport universal-cover (loops t) u ≡ t · u
  loops-to-x· t u =
    trans-universal-cover (loops t) u
    ∘ (ap (λ t' → transport (λ B → B) t' u) (β-nondep (Set _) FA x·-path t)
    ∘ trans-id-eq-to-path (_ , x·-is-equiv t) u)

{-
Here is an HIT declaration for the Cayley graph of the free group over A:

data cayley : Set where
  z : FA → cayley
  e : (t : A) (u : FA) → z u ≡ z (t · u)

We will see that [cayley] is contractible.
We want to show that [tot-cover] has the same introduction and elimination
rules, so that we can prove that [tot-cover] is contractible too.
We do not need to actually have the type [cayley], it is enough to show
that [tot-cover] has the same rules and then we can copy the proof of the
contractibility using the new rules.
-}

-- Introduction rules
CA-z : FA → tot-cover
CA-z u = (baseWA , u)

CA-e : (t : A) (u : FA) → CA-z u ≡ CA-z (t · u)
CA-e t u = Σ-eq (loops t) (loops-to-x· t u)

-- Elimination rule
module equivCA
  {i}
  (P : tot-cover → Set i)
  (z : (u : FA) → P (CA-z u))
  (e : (t : A) (u : FA) → transport P (CA-e t u) (z u) ≡ z (t · u)) where

  CA-e' : (t : A) (u : FA)
    → CA-z u ≡ CA-z (transport universal-cover (loops t) u)
  CA-e' t u = Σ-eq (loops t) refl

  abstract
    e' : (t : A) (u : FA)
      → transport P (CA-e' t u) (z u)
        ≡ z (transport universal-cover (loops t) u)
    e' t u = (trans-totalpath universal-cover P {x = (baseWA , u)}
               {y = (baseWA , transport universal-cover (loops t) u)} (loops t)
               refl z
             ∘ move!-transp-left (λ z → P (baseWA , z)) _ (loops-to-x· t u)
                                 (z (t · u))
             (! (trans-totalpath universal-cover P
                  {x = (baseWA , u)} {y = (baseWA , (t · u))}
                  (loops t) (loops-to-x· t u) z)
              ∘ e t u))
              ∘ apd z (! (loops-to-x· t u))

  P-base : (u : universal-cover (baseWA)) → P (baseWA , u)
  P-base u = z u

  abstract
    P-loops : (t : A) (u : universal-cover (baseWA))
      → transport (λ x → (t : universal-cover x) → P (x , t)) (loops t) P-base u
        ≡ P-base u
    P-loops t u =
      transport (λ u → transport (λ x → (t : universal-cover x) → P (x , t))
                                 (loops t) P-base u ≡ P-base u)
        (trans-trans-opposite universal-cover (loops t) u)
        (! (trans-totalpath universal-cover P
             {x = (baseWA , transport universal-cover (! (loops t)) u)}
             {y = (baseWA , transport universal-cover (loops t)
               (transport universal-cover (! (loops t)) u))}
             (loops t) refl z)
        ∘ e' t (transport universal-cover (! (loops t)) u))

  P-CA-rec : (x : WA) → (t : universal-cover x) → P (x , t)
  P-CA-rec = wedge-circles-rec (λ x → (t : universal-cover x) → P (x , t))
                               P-base (λ t → funext (P-loops t))

  -- Here is the conclusion of the elimination rule
  abstract
    CA-rec : (t : tot-cover) → P t
    CA-rec (x , y) = P-CA-rec x y
